# Exponential Distribution

$ f(x)=\left\{\begin{array}{cc}\lambda e^{-\lambda x}, & x \geq 0 \\ 0 & , x<0\end{array}\right. $

$ \mathrm{F}(x)=\int_{-\infty}^{x} f(y) d y=\left\{\begin{array}{cl}1-e^{-\lambda x} & , x \geq 0 \\ 0 & , x<0\end{array}\right. $

$ \begin{array}{l}P\{X \leq x\}=1-e^{-\lambda x} \\ P\{X>x\}=1-P\{X \leq x\}=e^{-\lambda x}\end{array} $



## Example:

Let $T$ as Exponential RV with parameter $\alpha $:

$ \int_{0}^{\infty} e^{-\alpha x} E[R(x)] d x=E\left[\int_{0}^{T} R(x) d x\right] $

Proof:

$ \begin{aligned} &E\left[\int_{0}^{\infty} R(x) I(x) d x\right] \\ 
& =\int_{0}^{\infty} E[R(x) I(x)] d x \\ & =\int_{0}^{\infty} E[R(x)] E[I(x)] d x \\ & =\int_{0}^{\infty} E[R(x)] P\{T \geq x\} d x \\ & =\int_{0}^{\infty} e^{-\alpha x} E[R(x)] d x\end{aligned} $

## Markov property

$ P\{X>s+t \mid X>t\}=P\{X>s\} $

Other form:

$ \frac{P\{X>s+t, X>t\}}{P\{X>t\}}=P\{X>s\} $

$ P\{X>s+t\}=P\{X>t\} P\{X>s\} $



