# $P_{ij}(t)$

$ 1-P_{i i}(h)=\sum_{j \neq i} P_{i j}(h)=v_{i} h+o(h) $

Then we get:

$ v_{i}=\lim _{h \rightarrow 0} \frac{1-P_{i i}(h)}{h} $

---

$ P_{i j}(h)=P_{i j} \cdot\left(v_{i} h+o(h)\right)+o(h)=P_{i j} v_{i} h+o(h) $

Then we get:

$ P_{i j}=\lim _{h \rightarrow 0} \frac{P_{i j}(h)}{v_{i} h}=\lim _{h \rightarrow 0} \frac{P_{i j}(h)}{1-P_{i i}(h)} $

# $q_{ij}$

$ q_{i j}=v_{i} P_{i j} $

$ v_{i}=v_{i} \sum_{j} P_{i j}=\sum_{j} v_{i} P_{i j}=\sum_{j} q_{i j} $

$ P_{i j}=\frac{q_{i j}}{v_{i}}=\frac{q_{i j}}{\sum_{j} q_{i j}} $

## CK Formula

$ P_{i j}(t+s)=\sum_{k=0}^{\infty} P_{i k}(t) P_{k j}(s) $

# Kolmogorov Backward Equation

For all states $ i, j $ and time $ t \geq 0 $,
$$
P_{i j}^{\prime}(t)=\sum_{k \neq i} q_{i k} P_{k j}(t)-v_{i} P_{i j}(t)
$$
where:
- $ P_{i j}(t) $ is the transition probability from state $ i $ to $ j $ by time $ t $,
- $ q_{i k} $ is the entry of the infinitesimal generator matrix $ Q\left(q_{i k}=v_{i} P_{i k}\right. $ for $ \left.k \neq i\right) $,
- $ v_{i}=-q_{i i} $ is the exit rate from state $ i $.

## Proof

$$
P_{i j}(t+h)=\sum_{k} P_{i k}(h) P_{k j}(t)
$$

Separate the sum:
$$
P_{i j}(t+h)=P_{i i}(h) P_{i j}(t)+\sum_{k \neq i} P_{i k}(h) P_{k j}(t)
$$

Substitute asymptotic expressions:
$$
P_{i j}(t+h)=\left(1-v_{i} h+o(h)\right) P_{i j}(t)+\sum_{k \neq i}\left(q_{i k} h+o(h)\right) P_{k j}(t)
$$

Expand:
$$
P_{i j}(t+h)=P_{i j}(t)-v_{i} h P_{i j}(t)+h \sum_{k \neq i} q_{i k} P_{k j}(t)+o(h)
$$

Rearrange:
$$
\frac{P_{i j}(t+h)-P_{i j}(t)}{h}=\sum_{k \neq i} q_{i k} P_{k j}(t)-v_{i} P_{i j}(t)+\frac{o(h)}{h}
$$

Take limit $ h \rightarrow 0 $ :
$$
\lim _{h \rightarrow 0} \frac{P_{i j}(t+h)-P_{i j}(t)}{h}=P_{i j}^{\prime}(t)=\sum_{k \neq i} q_{i k} P_{k j}(t)-v_{i} P_{i j}(t)
$$

# Pure birth euqation 

$ P_{i j}^{\prime}(t)=\lambda_{i} P_{i+1, j}(t)-\lambda_{i} P_{i j}(t) $

# Birth-death equation

$ P_{0 j}^{\prime}(t)=\lambda_{0} P_{1 j}(t)-\lambda_{0} P_{0 j}(t)=\lambda_{0}\left(P_{1 j}(t)-P_{0 j}(t)\right) $,

$ \begin{array}{c}P_{0 j}^{\prime}(t)=\lambda_{0} P_{1 j}(t)-\lambda_{0} P_{0 j}(t)=\lambda_{0}\left(P_{1 j}(t)-P_{0 j}(t)\right) \\ P_{i j}^{\prime}(t)=\left(\lambda_{i}+\mu_{i}\right)\left[\frac{\lambda_{i}}{\lambda_{i}+\mu_{i}} P_{i+1, j}(t)+\frac{\mu_{i}}{\lambda_{i}+\mu_{i}} P_{i-1, j}(t)\right]-\left(\lambda_{i}+\mu_{i}\right) P_{i j}(t), \mathrm{i}>0\end{array} $

# Kolmogorov Forward Equation

For most continuous-time Markov chains, the transition probabilities satisfy for all states $ i, j $ and time $ t \geq 0 $ :
$$
P_{i j}^{\prime}(t)=\sum_{k \neq j} P_{i k}(t) q_{k j}-P_{i j}(t) v_{j}
$$
where $ q_{k j} $ are entries of the infinitesimal generator matrix $ Q $, and $ v_{j}=-q_{j j} $ is the exit rate from state $ j $.

## Proof

Step 1: Chapman-Kolmogorov Equation
$$
P_{i j}(t+h)=\sum_{k} P_{i k}(t) P_{k j}(h) .
$$

Step 2: Separate the \( j \)-Term
$$
P_{i j}(t+h)=P_{i j}(t) P_{j j}(h)+\sum_{k \neq j} P_{i k}(t) P_{k j}(h) .
$$

Step 3: Asymptotic Behavior as \( h \rightarrow 0 \)
- \( P_{j j}(h)=1-v_{j} h+o(h) \),
- \( P_{k j}(h)=q_{k j} h+o(h) \) for \( k \neq j \).

Substitute:
$$
P_{i j}(t+h)=P_{i j}(t)\left(1-v_{j} h+o(h)\right)+\sum_{k \neq j} P_{i k}(t)\left(q_{k j} h+o(h)\right) .
$$

Step 4: Expand and Rearrange
$$
P_{i j}(t+h)=P_{i j}(t)-v_{j} h P_{i j}(t)+h \sum_{k \neq j} P_{i k}(t) q_{k j}+o(h) .
$$

Step 5: Form the Derivative
$$
\frac{P_{i j}(t+h)-P_{i j}(t)}{h}=\sum_{k \neq j} P_{i k}(t) q_{k j}-v_{j} P_{i j}(t)+\frac{o(h)}{h} .
$$

Step 6: Take Limit \( h \rightarrow 0 \)
$$
\lim _{h \rightarrow 0} \frac{P_{i j}(t+h)-P_{i j}(t)}{h}=P_{i j}^{\prime}(t)=\sum_{k \neq j} P_{i k}(t) q_{k j}-v_{j} P_{i j}(t) .
$$

# Pure birth equation 

For a pure birth process, the transition probabilities satisfy:
$$
\begin{array}{c}
P_{i i}^{\prime}(t)=-\lambda_{i} P_{i i}(t) \\
P_{i j}^{\prime}(t)=\lambda_{j-1} P_{i, j-1}(t)-\lambda_{j} P_{i j}(t), \quad j \geq i+1
\end{array}
$$
with initial conditions:
$$
\begin{array}{c}
P_{i i}(0)=1 \\
P_{i j}(0)=0, \quad j \neq i
\end{array}
$$

The solution to these differential equations is (recursively):
$$
\begin{array}{c}
P_{i i}(t)=e^{-\lambda_{i} t}, \quad i \geq 0 \\
P_{i i}(t)=\lambda_{i-1} e^{-\lambda_{j} t} \int_{0}^{t} e^{\lambda_{j} s} P_{i, j-1}(s) d s, \quad j \geq i+1
\end{array}
$$

## Proof 

Step 1: Prove \( P_{i i}(t)=e^{-\lambda_{i} t} \)
- Differential Equation:
$$
P_{i i}^{\prime}(t)=-\lambda_{i} P_{i i}(t), \quad P_{i i}(0)=1 .
$$
- Solution:

This is a first-order linear ODE. Separating variables:
$$
\frac{d P_{i i}}{P_{i i}}=-\lambda_{i} d t \Longrightarrow \ln P_{i i}=-\lambda_{i} t+C
$$

Apply \( P_{i i}(0)=1 \) :
$$
\ln 1=0+C \Longrightarrow C=0 \Longrightarrow P_{i i}(t)=e^{-\lambda_{i} t} \text {. }
$$

Step 2: Prove \( P_{i j}(t)=\lambda_{j-1} e^{-\lambda_{j} t} \int_{0}^{t} e^{\lambda_{j} s} P_{i, j-1}(s) d s \) for \( j \geq i+1 \)
- Differential Equation:
$$
P_{i j}^{\prime}(t)=\lambda_{j-1} P_{i, j-1}(t)-\lambda_{j} P_{i j}(t), \quad P_{i j}(0)=0 . \quad(j \geq i+1)
$$
- Solution:

Rewrite as a first-order linear nonhomogeneous ODE:
$$
P_{i j}^{\prime}(t)+\lambda_{j} P_{i j}(t)=\lambda_{j-1} P_{i, j-1}(t)
$$

Multiply by the integrating factor \( e^{\lambda_{j} t} \) :
$$
e^{\lambda_{j} t} P_{i j}^{\prime}(t)+\lambda_{j} e^{\lambda_{j} t} P_{i j}(t)=\lambda_{j-1} P_{i, j-1}(t) e^{\lambda_{j} t}
$$

The left side is the derivative of \( e^{\lambda_{j} t} P_{i j}(t) \) :
$$
\frac{d}{d t}\left[e^{\lambda_{j} t} P_{i j}(t)\right]=\lambda_{j-1} P_{i, j-1}(t) e^{\lambda_{j} t}
$$

Integrate both sides from 0 to \( t \) :
$$
e^{\lambda_{j} t} P_{i j}(t)-\underbrace{e^{0} P_{i j}(0)}_{=0}=\lambda_{j-1} \int_{0}^{t} e^{\lambda_{j} s} P_{i, j-1}(s) d s
$$

Solve for \( P_{i j}(t) \) :
$$
P_{i j}(t)=\lambda_{j-1} e^{-\lambda_{j} t} \int_{0}^{t} e^{\lambda_{j} s} P_{i, j-1}(s) d s
$$

Step 3: Verify Initial Conditions
- For \( P_{\mathrm{i} i}(t) \) :
$$
P_{i i}(0)=e^{-\lambda_{i} \cdot U}=e^{U}=1
$$
- For \( P_{i j}(t)(j \neq i) \) :
$$
P_{i j}(0)=\lambda_{j-1} e^{0} \int_{0}^{U} e^{\lambda_{j} s} P_{i, j-1}(s) d s=0
$$
- The solution satisfies \( P_{i j}(0)=0 \) for \( j \neq i \).

# Birth-death equation

For a general birth-death process, the forward Kolmogorov equations are:
$$
\begin{array}{c}
P_{i 0}^{\prime}(t)=\sum_{k \neq 0} q_{k 0} P_{i k}(t)-\lambda_{0} P_{i 0}(t)=\mu_{1} P_{i 1}(t)-\lambda_{0} P_{i 0}(t) \\
P_{i j}^{\prime}(t)=\sum_{k \neq j} q_{k j} P_{i k}(t)-\left(\lambda_{j}+\mu_{j}\right) P_{i j}(t)=\lambda_{j-1} P_{i, j-1}(t) \\
\quad+\mu_{j+1} P_{i, j+1}(t)-\left(\lambda_{j}+\mu_{j}\right) P_{i j}(t)
\end{array}
$$


